src/program_proof/mpaxos/marshal_proof.v
@@ -475,9 +475,9 @@ Proof.
   iFrame. iExists _; by iFrame "∗#".
 Qed.
 
-Lemma wp_decode sl st :
+Lemma wp_decode sl st q :
   {{{
-        own_slice_small sl byteT 1 (encode st)
+        own_slice_small sl byteT q (encode st)
   }}}
     decodePaxosState (slice_val sl)
   {{{
@@ -497,7 +497,8 @@ Proof.
   wp_load. wp_apply (wp_ReadInt with "[$]"). iIntros (?) "?".
   wp_pures. wp_storeField. wp_store.
   wp_load. wp_apply (wp_ReadInt with "[$]"). iIntros (?) "Hsl".
-  iMod (readonly_alloc_1 with "Hsl") as "#Hsl".
+  iMod (readonly_alloc (own_slice_small s'2 byteT 1 st.(state)) with "[Hsl]") as "#Hsl".
+  { done. }
   wp_pures. wp_store. wp_storeField. wp_load. wp_pures. wp_storeField.
   iApply "HΦ".
   iModIntro. repeat iExists _; iFrame "∗#".
